Performant_Isabelle_ML.thy
@@ -3,10 +3,11 @@ theory Performant_Isabelle_ML
 begin
 
 ML_file \<open>library/improved_net.ML\<close>
+ML_file \<open>library/inet_collection.ML\<close>
+ML_file \<open>library/pattern.ML\<close>
 ML_file \<open>library/merely_rewrite.ML\<close>
 ML_file \<open>library/hash_table.ML\<close>
 ML_file \<open>library/term_size.ML\<close>
-ML_file \<open>library/pattern.ML\<close>
 
 (* MessagePack serialization library (mlmsgpack), relocated here from Isabelle_RPC
    so it is reachable by any session based on Performant_Isabelle_ML
