Skel_Smoke.thy
@@ -2,5 +2,6 @@ theory Skel_Smoke
   imports Main
 begin
 ML_file \<open>library/improved_net.ML\<close>
+ML_file \<open>library/pattern.ML\<close>
 ML_file \<open>library/merely_rewrite.ML\<close>
 end
